refinedVST/typing/exist.v
@@ -103,12 +103,12 @@ Section tyexist.
     SimpleSubsumePlace ty1 (x @ tyexists ty2) P.
   Proof. iIntros (l β) "HP Hl". rewrite ! tyexists_eq. iApply (@simple_subsume_place with "HP Hl"). Qed.
 
-  Global Program Instance tyexist_optional x cty (ty : A → _) optty ot1 ot2
-    `{!∀ x, Optionable cty (ty x) optty ot1 ot2} : Optionable cty (x @ tyexists ty) optty ot1 ot2 := {|
+  Global Program Instance tyexist_optional x cty cty2 (ty : A → _) optty ot1 ot2
+    `{!∀ x, Optionable cty cty2 (ty x) optty ot1 ot2} : Optionable cty cty2 (x @ tyexists ty) optty ot1 ot2 := {|
     opt_pre v1 v2 := opt_pre (ty x) v1 v2
   |}.
   Next Obligation.
-    move => ????????????. rewrite {1}/ty_own_val_at {1}/ty_own_val/= ty_exists_rty_eq /ty_has_op_type /ty_own_val_at /ty_own_val. apply opt_bin_op.
+    move => ?????????????. rewrite {1}/ty_own_val_at {1}/ty_own_val/= ty_exists_rty_eq /ty_has_op_type /ty_own_val_at /ty_own_val. apply opt_bin_op.
   Qed.
 
   Global Instance optionable_agree_tyexists (ty2 : A → type) ty1
